fix: use height for define it as Prop

LeanYjs/ItemOrder.lean
@@ -3,43 +3,37 @@ import LeanYjs.ActorId
 import LeanYjs.ItemOriginOrder
 
 import Mathlib.Tactic.ApplyAt
+import Mathlib.Data.Nat.Basic
+
+def max4 (x y z w : Nat) : Nat :=
+  max (max x y) (max z w)
 
 mutual
-inductive YjsLt {A : Type} : YjsPtr A -> YjsPtr A -> Type where
-  | ltConflict i1 i2 : ConflictLt i1 i2 -> YjsLt i1 i2
-  | ltOriginOrder i1 i2 : OriginLt _ i1 i2 -> YjsLt i1 i2
-  | ltTrans x y z: YjsLt x y -> YjsLt y z -> YjsLt x z
+inductive YjsLt {A : Type} : Nat -> YjsPtr A -> YjsPtr A -> Prop where
+  | ltConflict h i1 i2 : ConflictLt h i1 i2 -> YjsLt (h + 1) i1 i2
+  | ltOriginOrder i1 i2 : OriginLt _ i1 i2 -> YjsLt 0 i1 i2
+  | ltTrans h1 h2 x y z: YjsLt h1 x y -> YjsLt h2 y z -> YjsLt (max h1 h2 + 1) x z
 
-inductive ConflictLt {A : Type} : YjsPtr A -> YjsPtr A -> Type where
-  | ltOriginDiff : forall l1 l2 r1 r2 id1 id2 c1 c2,
-    YjsLt l2 l1
-    -> YjsLt (YjsItem.item l1 r1 id1 c1) r2
-    -> YjsLt l1 (YjsItem.item l2 r2 id2 c2)
-    -> YjsLt (YjsItem.item l2 r2 id2 c2) r1
-    -> ConflictLt (YjsItem.item l1 r1 id1 c1) (YjsItem.item l2 r2 id2 c2)
-  | ltOriginSame : forall l r1 r2 id1 id2 (c1 c2 : A),
-    YjsLt (YjsItem.item l r1 id1 c1) r2
-    -> YjsLt (YjsItem.item l r2 id2 c2) r1
+inductive ConflictLt {A : Type} : Nat -> YjsPtr A -> YjsPtr A -> Prop where
+  | ltOriginDiff h1 h2 h3 h4 l1 l2 r1 r2 id1 id2 c1 c2 :
+    YjsLt h1 l2 l1
+    -> YjsLt h2 (YjsItem.item l1 r1 id1 c1) r2
+    -> YjsLt h3 l1 (YjsItem.item l2 r2 id2 c2)
+    -> YjsLt h4 (YjsItem.item l2 r2 id2 c2) r1
+    -> ConflictLt (max4 h1 h2 h3 h4 + 1) (YjsItem.item l1 r1 id1 c1) (YjsItem.item l2 r2 id2 c2)
+  | ltOriginSame h1 h2 l r1 r2 id1 id2 (c1 c2 : A) :
+    YjsLt h1 (YjsItem.item l r1 id1 c1) r2
+    -> YjsLt h2 (YjsItem.item l r2 id2 c2) r1
     -> id1 < id2
-    -> ConflictLt (YjsItem.item l r1 id1 c1) (YjsItem.item l r2 id2 c2)
+    -> ConflictLt (max h1 h2 + 1) (YjsItem.item l r1 id1 c1) (YjsItem.item l r2 id2 c2)
 end
 
-mutual
-def YjsLt.height {A} {x y : YjsPtr A} : YjsLt x y -> Nat
-  | YjsLt.ltConflict i1 i2 h => h.height
-  | YjsLt.ltOriginOrder i1 i2 _ => 1
-  | YjsLt.ltTrans x _ z lt1 lt2 => max (YjsLt.height lt1) (YjsLt.height lt2) + 1
-
-def ConflictLt.height {A} {x y : YjsPtr A} : ConflictLt x y -> Nat
-  | ConflictLt.ltOriginDiff l1 l2 r1 r2 id1 id2 c1 c2 h1 h2 h3 h4 =>
-    max h1.height (max h2.height (max h3.height h4.height)) + 1
-  | ConflictLt.ltOriginSame l r1 r2 id1 id2 c1 c2 h1 h2 h3 =>
-    max h1.height h2.height + 1
-end
+def YjsLeq {A : Type} (h : Nat) (x y : YjsPtr A) : Prop :=
+  x = y ∨ YjsLt h x y
 
 inductive LtSequence {A : Type} : YjsPtr A -> YjsPtr A -> List (YjsPtr A) -> Prop where
   | base : forall x, LtSequence x x []
-  | step1 : forall x y z is, ConflictLt x y -> LtSequence y z is -> LtSequence x z (y :: is)
+  | step1 : forall x y z is h, ConflictLt h x y -> LtSequence y z is -> LtSequence x z (y :: is)
   | step2 : forall x y z is, OriginLt _ x y -> LtSequence y z is -> LtSequence x z (y :: is)
 
 lemma LtSequenceConcat {A : Type} {x y z : YjsPtr A} {is1 is2 : List (YjsPtr A)} :
@@ -49,38 +43,51 @@ lemma LtSequenceConcat {A : Type} {x y z : YjsPtr A} {is1 is2 : List (YjsPtr A)}
     | base x =>
       intros lt2
       apply lt2
-    | step1 x y z is lt1 lt2 ih =>
+    | step1 x y z is _ lt1 lt2 ih =>
       intros lt
       apply LtSequence.step1 <;> try assumption
-      apply ih <;> assumption
+      apply ih
+      assumption
     | step2 x y z is lt1 lt2 ih =>
       intros lt
       apply LtSequence.step2 <;> try assumption
-      apply ih <;> assumption
+      apply ih
+      assumption
 
-
-def YjsLtSequence (A : Type) : forall (x y : YjsPtr A), YjsLt x y ->
-  ∃ is : List (YjsPtr A), LtSequence x y is := fun x y lt =>
+mutual
+def YjsLtSequence (A : Type) : forall (x y : YjsPtr A) h, YjsLt h x y ->
+  ∃ is : List (YjsPtr A), LtSequence x y is := by
+    intros x y h
+    apply Nat.strongRecOn' (P := fun h => ∀ x y, YjsLt h x y -> ∃ is : List (YjsPtr A), LtSequence x y is)
+    intros h' ih x y lt
     match lt with
-    | YjsLt.ltConflict x y _ => by
+    | YjsLt.ltConflict h x y _ =>
       apply Exists.intro [y]
       apply LtSequence.step1 <;> try assumption
       apply LtSequence.base
-    | YjsLt.ltOriginOrder x y _ => by
+    | YjsLt.ltOriginOrder x y _ =>
       apply Exists.intro [y]
       apply LtSequence.step2 <;> try assumption
       apply LtSequence.base
-    | YjsLt.ltTrans _ z _  lt1 lt2 =>
-      have h : lt1.height < (YjsLt.ltTrans x z _ lt1 lt2).height := by
-        simp [YjsLt.height]
+    | YjsLt.ltTrans h1 h2 _ z _  lt1 lt2 =>
+      -- have h : lt1.height < (YjsLt.ltTrans x z _ lt1 lt2).height := by
+      --   simp [YjsLt.height]
+      --   omega
+      have hlt1 : h1 < max h1 h2 + 1 := by
         omega
-      match YjsLtSequence A x z lt1 with
+      match ih h1 hlt1 x z lt1 with
       | Exists.intro is1 lt1' =>
-        have h : lt2.height < (YjsLt.ltTrans x z _ lt1 lt2).height := by
-          simp [YjsLt.height]
+        -- have h : lt2.height < (YjsLt.ltTrans x z _ lt1 lt2).height := by
+        --   simp [YjsLt.height]
+        --   omega
+        have hlt2 : h2 < max h1 h2 + 1 := by
           omega
-        match YjsLtSequence A z y lt2 with
-        | Exists.intro is2 lt2 => by
+        match ih h2 hlt2 z y lt2 with
+        | Exists.intro is2 lt2 =>
           apply Exists.intro (is1 ++ is2)
           apply LtSequenceConcat <;> try assumption
-    termination_by x y lt => lt.height
+end
+
+lemma YjsInvariant A h (x y : YjsItem A) :
+  @YjsLt A h x y -> ∃ h1, @YjsLeq A h1 x (y.origin) ∨ @YjsLeq A h1 (y.origin) (x.origin) := by
+  sorry
