LeanYjs/Integrate.lean
@@ -1,6 +1,7 @@
-import LeanYjs.YItem
+import LeanYjs.Item
 import LeanYjs.ActorId
-import LeanYjs.ItemPartialOrder
+import LeanYjs.ItemOriginOrder
+import LeanYjs.ItemOrder
 
 inductive IntegrateError where
 | notFound : IntegrateError
@@ -62,10 +63,10 @@ inductive ArrayPairwise {α : Type} (f : α -> α -> Prop) : Array α -> Prop wh
   ArrayPairwise f arr -> (forall b: α, b ∈ arr -> f b a)
   -> ArrayPairwise f (Array.push arr a) -- if the tail is pairwise, then adding an element is pairwise
 
-theorem integrate_sound (A: Type) [BEq A] (newItem : YjsItem A) (arr newArr : Array (YjsItem A)) :
-  ArrayPairwise (fun (x y : YjsItem A) => @YjsLt A x y) arr
+theorem integrate_sound (A: Type) [BEq A] (newItem : YjsItem A) (arr newArr : Array (YjsItem A)) h1 :
+  ArrayPairwise (fun (x y : YjsItem A) => @YjsLt A h1 x y) arr
   -> integrate newItem arr = Except.ok newArr
-  -> ArrayPairwise (fun (x y : YjsItem A) => @YjsLt A x y) newArr := by
+  -> ∃ h2, ArrayPairwise (fun (x y : YjsItem A) => @YjsLt A h2 x y) newArr := by
   sorry
 
 theorem integrate_commutative (A: Type) [BEq A] (a b : YjsItem A) (arr1 arr2 arr3 arr2' arr3' : Array (YjsItem A)) :
